theories/PartitionedPolicies/PartitionedEDF.v
@@ -1,4 +1,4 @@
-From Stdlib Require Import Arith Arith.PeanoNat Lia.
+From Stdlib Require Import Arith Arith.PeanoNat Lia List Bool.
 Require Import Base.
 Require Import ScheduleModel.
 Require Import SchedulerInterface.
@@ -7,6 +7,7 @@ Require Import SchedulingAlgorithmSchedulerBridge.
 Require Import Partitioned.
 Require Import PartitionedCompose.
 Require Import UniPolicies.EDF.
+Require Import UniPolicies.EDFOptimality.
 
 (* Fully constructive: no Classical import. *)
 
@@ -81,4 +82,83 @@ Proof.
   intros c Hlt.
   unfold edf_scheduler.
   exact (Hlocal c Hlt).
+Qed.
+
+Definition local_jobset_bool
+    (assign : JobId -> CPU)
+    (J_bool : JobId -> bool)
+    (c : CPU) : JobId -> bool :=
+  fun j => andb (J_bool j) (Nat.eqb (assign j) c).
+
+Lemma local_jobset_bool_spec :
+    forall (assign : JobId -> CPU)
+           (J : JobId -> Prop)
+           (J_bool : JobId -> bool)
+           c,
+      (forall x, J_bool x = true <-> J x) ->
+      forall x,
+        local_jobset_bool assign J_bool c x = true <->
+        local_jobset assign J c x.
+Proof.
+  intros assign J J_bool c HJbool x.
+  unfold local_jobset_bool, local_jobset.
+  split.
+  - intro Hx.
+    apply andb_prop in Hx.
+    destruct Hx as [HJx Hassign].
+    apply Nat.eqb_eq in Hassign.
+    apply HJbool in HJx.
+    tauto.
+  - intros [HJx Hassign].
+    apply <- HJbool in HJx.
+    apply Nat.eqb_eq in Hassign.
+    rewrite HJx, Hassign.
+    reflexivity.
+Qed.
+
+Theorem partitioned_edf_schedulable_by_on_of_local_feasible :
+    forall (assign : JobId -> CPU) (m : nat)
+           (valid_assignment : forall j, assign j < m)
+           (J : JobId -> Prop)
+           (J_bool : JobId -> bool)
+           enumJ jobs,
+      (forall x, J_bool x = true <-> J x) ->
+      (forall j, J j -> In j enumJ) ->
+      (forall j, In j enumJ -> J j) ->
+      (forall c, c < m ->
+        feasible_on (local_jobset assign J c) jobs 1) ->
+      schedulable_by_on
+        J
+        (partitioned_edf_scheduler m (enum_local_candidates_of assign enumJ))
+        jobs m.
+Proof.
+  intros assign m valid_assignment J J_bool enumJ jobs
+         HJbool Henum_complete Henum_sound Hlocal_feasible.
+  eapply (local_edf_schedulable_by_on_implies_partitioned_edf_schedulable_by_on
+            assign m valid_assignment J
+            (enum_local_candidates_of assign enumJ)).
+  - intros c Hlt.
+    exact (enum_local_candidates_spec assign m J enumJ
+             Henum_complete Henum_sound c Hlt).
+  - intros c Hlt.
+    eapply (edf_optimality_on_finite_jobs
+              (local_jobset assign J c)
+              (local_jobset_bool assign J_bool c)
+              (local_candidates assign enumJ c)
+              (enum_local_candidates_of assign enumJ c)).
+    + exact (enum_local_candidates_spec assign m J enumJ
+               Henum_complete Henum_sound c Hlt).
+    + intros x.
+      exact (local_jobset_bool_spec assign J J_bool c HJbool x).
+    + intros j Hj.
+      exact (local_candidates_complete assign J enumJ
+               Henum_complete j c (proj1 Hj) (proj2 Hj)).
+    + intros j Hin.
+      split.
+      * apply Henum_sound.
+        unfold local_candidates in Hin.
+        apply filter_In in Hin.
+        exact (proj1 Hin).
+      * exact (local_candidates_sound assign enumJ c j Hin).
+    + exact (Hlocal_feasible c Hlt).
 Qed.
